Find the first order and second order weak derivatives for the following function $u: R \rightarrow R$, if exists:

\begin{enumerate}
\item
  $$
  u(x) =
  \begin{cases}
    1 - |x| & |x| \leq 1\\
    0 & |x| > 1
  \end{cases}
  $$

  The first order weak derivative is
  $$
  Du(x) =
  \begin{cases}
    1 & -1 < x < 0\\
    -1 & 0 < x < 1\\
    0 & \text{otherwise}
  \end{cases}
  $$
  The second order weak derivative doesn't exist.
  We can prove this by working backwards and using the uniqueness of the weak derivative to prove our claim.
  We need to show that $\int_R Du \phi \dx = -\int_R u \phi' \dx$ for any $\phi \in C_C^\infty(R)$.
  To do so, we simply note that $\deriv{}{x}(1 + x) = 1$ and $\deriv{}{x}(1 - x) = -1$,
  which is nice since we need these to be $0$ at the $-1$ and $1$, respectively, while having the same value at $0$.
  Then integrating by parts results in:
  \begin{align*}
    \int Du(x) \phi(x) = &\int_{-1}^0 \phi(x) \dx - \int_0^1 \phi(x) \dx\\
                       = &\phi(x) (1 + x) \bigg\rvert_{x=-1}^{0} - \int_{-1}^0 (1 + x) \phi'(x)
                          + \phi(x) (1 - x) \bigg\rvert_{x=0}^{1} - \int_0^1 (1 - x) \phi'(x) \dx\\
                       = &\phi(0) - \int_{-1}^0 (1 + x) \phi'(x) - \phi(0) - \int_0^1 (1 - x) \phi'(x) \dx\\
                       = &-\int_{-1}^0 (1 + x) \phi'(x) - \int_0^1 (1 - x) \phi'(x) \dx
                       = -\int_{-1}^0 (1 - |x|) \phi'(x) - \int_0^1 (1 - |x|) \phi'(x) \dx\\
                       = &-\int_{-1}^1 (1 - |x|) \phi'(x)
  \end{align*}

  Thus, $Du$ is the weak derivative of $u$.

\item
  $$
  u(x) = |\sin(x)|
  $$

  First we rewrite this in cases:
  $$
  u(x) =
  \begin{cases}
    \sin(x) & k \pi < x < (k + 1) \pi\\
    -\sin(x) & (k + 1) \pi < x < (k + 2) \pi
  \end{cases}
  $$

  Then the first order weak derivative is
  $$
  Du(x) =
  \begin{cases}
    \cos(x) & k \pi < x < (k + 1) \pi\\
    -\cos(x) & (k + 1) \pi < x < (k + 2) \pi
  \end{cases}
  $$

  The second order weak derivative is
  $$
  D^2u(x) =
  \begin{cases}
    -\sin(x) & k \pi < x < (k + 1) \pi\\
    \sin(x) & (k + 1) \pi < x < (k + 2) \pi
  \end{cases}
  $$
  which is just $-|\sin(x)| = -u(x)$

\end{enumerate}
